veric/binop_lemmas.v
@@ -8,393 +8,136 @@ Require Import veric.Clight_lemmas.
 Require Import veric.expr.
 Import Cop.
 
-Lemma typecheck_add_sound:
-forall (Delta : tycontext) (rho : environ) (e1 e2 : expr) (t : type),
-   denote_tc_assert (typecheck_expr Delta e2) rho ->
-   denote_tc_assert (isBinOpResultType Oadd e1 e2 t) rho ->
-   denote_tc_assert (typecheck_expr Delta e1) rho ->
-   typecheck_val (eval_expr e2 rho) (typeof e2) = true ->
-   typecheck_val (eval_expr e1 rho) (typeof e1) = true ->
-   typecheck_val
-     (eval_binop Oadd (typeof e1) (typeof e2) (eval_expr e1 rho)
-        (eval_expr e2 rho)) t = true.
-Proof. 
-intros. simpl in *; unfold eval_binop; unfold sem_binary_operation.
-unfold sem_add in *. 
-destruct (typeof e1); destruct (typeof e2); simpl in *; auto;
+Lemma typecheck_val_void:
+  forall v, typecheck_val v Tvoid = true -> False.
+Proof.
+destruct v; simpl; congruence.
+Qed.
 
-try destruct i; try destruct s; try destruct i0; try destruct s0; 
-try solve [simpl in *; try solve[inv H0]; unfold_coerce;
-tc_assert_ext; auto;
- destruct t; simpl in *; auto; unfold_coerce;
-destruct (eval_expr e1 rho); destruct (eval_expr e2 rho); auto;
-simpl in *; tc_assert_ext; auto].
-Qed. 
+Definition denote_tc_assert' (a: tc_assert) (rho: environ) : Prop.
+pose (P := denote_tc_assert a rho).
+unfold denote_tc_assert in P.
+super_unfold_lift.
+destruct a; apply P.
+Defined.
+
+Lemma denote_tc_assert'_eq:
+  denote_tc_assert' = denote_tc_assert.
+Proof.
+extensionality a rho.
+destruct a; reflexivity.
+Qed.
+
+Ltac typecheck_sound_solver Delta rho e1 e2 t :=
+ match goal with
+ | H: denote_tc_assert (typecheck_expr Delta e2) rho,
+   H0: denote_tc_assert (isBinOpResultType _ e1 e2 t) rho,
+   H1: typecheck_val (eval_expr e2 rho) (typeof e2) = true,
+   H2: typecheck_val (eval_expr e1 rho) (typeof e1) = true |- _ =>
+rewrite <- denote_tc_assert'_eq in *;
+simpl in *;
+ destruct (typeof e1) as [ | [ | | | ] [ | ]  | [ | ]  | | | | | | ]; 
+      try (contradiction H0);
+ destruct (typeof e2) as [ | [ | | | ] [ | ]  | [ | ]  | | | | | | ]; 
+      try (contradiction H0);
+ destruct t; try (contradiction H0);
+simpl in *;
+try solve [destruct (eval_expr e1 rho); inv H2;
+               destruct (eval_expr e2 rho); inv H1;
+               try (contradiction H0);
+               simpl; auto]
+end.
+
 
 Lemma typecheck_sub_sound:
 forall (Delta : tycontext) (rho : environ) (e1 e2 : expr) (t : type),
    denote_tc_assert (typecheck_expr Delta e2) rho ->
    denote_tc_assert (isBinOpResultType Osub e1 e2 t) rho ->
-   denote_tc_assert (typecheck_expr Delta e1) rho ->
    typecheck_val (eval_expr e2 rho) (typeof e2) = true ->
    typecheck_val (eval_expr e1 rho) (typeof e1) = true ->
    typecheck_val
      (eval_binop Osub (typeof e1) (typeof e2) (eval_expr e1 rho)
         (eval_expr e2 rho)) t = true.
 Proof. 
-intros. simpl in *; unfold eval_binop; unfold sem_binary_operation.
-unfold sem_sub in *. 
-destruct (typeof e1); destruct (typeof e2); simpl in *; auto;
+intros; typecheck_sound_solver Delta rho e1 e2 t;
+unfold tc_bool, eval_binop in *; simpl in *; unfold sem_sub; simpl;
+try (remember (Int.eq (Int.repr (sizeof t0)) Int.zero) as ez; destruct ez; simpl in *; auto);
+destruct (eval_expr e1 rho); inv H2; destruct (eval_expr e2 rho); inv H1; 
+ simpl in *; decompose [and] H0; try contradiction; auto;
+ destruct (zeq b b0); inv H3; simpl; auto.
+Qed.
 
-try destruct i; try destruct s; try destruct i0; try destruct s0; 
-simpl in *; try solve[inv H0]; unfold_coerce;
-try solve[
-destruct t; simpl in *; auto;
-try (remember (negb (Int.eq (Int.repr (sizeof t0)) Int.zero)); 
-unfold tc_bool in *; try if_tac in H0); simpl in *; unfold_coerce; tc_assert_ext; auto; 
-try solve [destruct (eval_expr e1 rho); destruct (eval_expr e2 rho); auto;
-simpl in *; tc_assert_ext; auto; repeat (if_tac; auto)]].
-Qed. 
- 
-Lemma typecheck_mul_sound:
-forall (Delta : tycontext) (rho : environ) (e1 e2 : expr) (t : type),
+Lemma typecheck_divmod_sound:
+forall op (Delta : tycontext) (rho : environ) (e1 e2 : expr) (t : type)
+   (OPER: match op with Odiv | Omod => True | _ => False end),
    denote_tc_assert (typecheck_expr Delta e2) rho ->
-   denote_tc_assert (isBinOpResultType Omul e1 e2 t) rho ->
-   denote_tc_assert (typecheck_expr Delta e1) rho ->
+   denote_tc_assert (isBinOpResultType op e1 e2 t) rho ->
+    denote_tc_assert (typecheck_expr Delta e1) rho ->
    typecheck_val (eval_expr e2 rho) (typeof e2) = true ->
    typecheck_val (eval_expr e1 rho) (typeof e1) = true ->
    typecheck_val
-     (eval_binop Omul (typeof e1) (typeof e2) (eval_expr e1 rho)
+     (eval_binop op (typeof e1) (typeof e2) (eval_expr e1 rho)
         (eval_expr e2 rho)) t = true.
 Proof. 
-intros. simpl in *; unfold eval_binop; unfold sem_binary_operation.
-unfold sem_sub in *. 
-destruct (typeof e1); destruct (typeof e2); simpl in *; auto;
+intros.
+destruct op; try contradiction;
+abstract (typecheck_sound_solver Delta rho e1 e2 t;
+(( destruct H0 as  [H0 H0']; hnf in H0,H0') ||
+(hnf in H0));
+destruct (eval_expr e1 rho); try contradiction;
+destruct (eval_expr e2 rho); try contradiction;
+unfold eval_binop, sem_binary_operation, sem_div, sem_mod;
+try (destruct (Int.eq i1 Int.zero); try (contradiction H0); simpl);
+try (destruct (Int.eq i0 (Int.repr Int.min_signed) && Int.eq i1 Int.mone);
+      inv H0');
+ simpl; auto).
+Qed.
 
-try destruct i; try destruct s; try destruct i0; try destruct s0; 
-simpl in *; try solve[inv H0]; unfold_coerce;
-tc_assert_ext; auto;
-destruct (eval_expr e1 rho); destruct (eval_expr e2 rho); auto;
-simpl in *; destruct t; simpl in *; auto; unfold_coerce; tc_assert_ext; auto; repeat (if_tac; auto). 
-Qed. 
-
-Lemma typecheck_div_sound:
-forall (Delta : tycontext) (rho : environ) (e1 e2 : expr) (t : type),
-   denote_tc_assert (typecheck_expr Delta e2) rho ->
-   denote_tc_assert (isBinOpResultType Odiv e1 e2 t) rho ->
-   denote_tc_assert (typecheck_expr Delta e1) rho ->
-   typecheck_val (eval_expr e2 rho) (typeof e2) = true ->
-   typecheck_val (eval_expr e1 rho) (typeof e1) = true ->
-   typecheck_val
-     (eval_binop Odiv (typeof e1) (typeof e2) (eval_expr e1 rho)
-        (eval_expr e2 rho)) t = true.
-Proof. 
-intros. simpl in *; unfold eval_binop; unfold sem_binary_operation.
-unfold sem_div in *. 
-destruct (typeof e1); destruct (typeof e2); simpl in *; auto;
-
-try destruct i; try destruct s; try destruct i0; try destruct s0; 
-simpl in *; try solve[inv H0]; unfold_coerce;
- destruct t; simpl in *; auto; unfold_coerce;
-tc_assert_ext; auto;
-destruct (eval_expr e1 rho); destruct (eval_expr e2 rho); auto;
-simpl in *;
-unfold_coerce; tc_assert_ext; auto; repeat (try rewrite orb_if; rewrite andb_if);
-repeat (if_tac; auto). 
-Qed. 
-
-Lemma typecheck_mod_sound:
-forall (Delta : tycontext) (rho : environ) (e1 e2 : expr) (t : type),
-   denote_tc_assert (typecheck_expr Delta e2) rho ->
-   denote_tc_assert (isBinOpResultType Omod e1 e2 t) rho ->
-   denote_tc_assert (typecheck_expr Delta e1) rho ->
-   typecheck_val (eval_expr e2 rho) (typeof e2) = true ->
-   typecheck_val (eval_expr e1 rho) (typeof e1) = true ->
-   typecheck_val
-     (eval_binop Omod (typeof e1) (typeof e2) (eval_expr e1 rho)
-        (eval_expr e2 rho)) t = true.
-Proof. 
-intros. simpl in *; unfold eval_binop; unfold sem_binary_operation.
-unfold sem_mod in *. 
-destruct (typeof e1); destruct (typeof e2); simpl in *; auto;
-
-try destruct i; try destruct s; try destruct i0; try destruct s0; 
-simpl in *; try solve[inv H0]; unfold_coerce;
-destruct t; simpl in *; auto; unfold_coerce;
-tc_assert_ext; auto;
-destruct (eval_expr e1 rho); destruct (eval_expr e2 rho); auto;
-simpl in *; unfold_coerce; tc_assert_ext; auto; repeat (try rewrite orb_if; rewrite andb_if);
-repeat (if_tac; auto). 
-Qed. 
-
-Lemma typecheck_and_sound:
-forall (Delta : tycontext) (rho : environ) (e1 e2 : expr) (t : type),
-   denote_tc_assert (typecheck_expr Delta e2) rho ->
-   denote_tc_assert (isBinOpResultType Oand e1 e2 t) rho ->
-   denote_tc_assert (typecheck_expr Delta e1) rho ->
-   typecheck_val (eval_expr e2 rho) (typeof e2) = true ->
-   typecheck_val (eval_expr e1 rho) (typeof e1) = true ->
-   typecheck_val
-     (eval_binop Oand (typeof e1) (typeof e2) (eval_expr e1 rho)
-        (eval_expr e2 rho)) t = true.
-Proof. 
-intros. simpl in *; unfold eval_binop; unfold sem_binary_operation.
-unfold sem_and in *. 
-destruct (typeof e1); destruct (typeof e2); simpl in *; auto;
-
-try destruct i; try destruct s; try destruct i0; try destruct s0; 
-simpl in *; try solve[inv H0]; unfold_coerce;
-tc_assert_ext; auto;
-destruct (eval_expr e1 rho); destruct (eval_expr e2 rho); auto;
-simpl in *; destruct t; simpl in *; auto; unfold_coerce;
- tc_assert_ext; auto; repeat (try rewrite orb_if; rewrite andb_if);
-repeat (if_tac; auto). 
-Qed. 
-
-Lemma typecheck_or_sound:
-forall (Delta : tycontext) (rho : environ) (e1 e2 : expr) (t : type),
-   denote_tc_assert (typecheck_expr Delta e2) rho ->
-   denote_tc_assert (isBinOpResultType Oor e1 e2 t) rho ->
-   denote_tc_assert (typecheck_expr Delta e1) rho ->
-   typecheck_val (eval_expr e2 rho) (typeof e2) = true ->
-   typecheck_val (eval_expr e1 rho) (typeof e1) = true ->
-   typecheck_val
-     (eval_binop Oor (typeof e1) (typeof e2) (eval_expr e1 rho)
-        (eval_expr e2 rho)) t = true.
-Proof. 
-intros. simpl in *; unfold eval_binop; unfold sem_binary_operation.
-unfold sem_or in *. 
-destruct (typeof e1); destruct (typeof e2); simpl in *; auto;
-
-try destruct i; try destruct s; try destruct i0; try destruct s0; 
-simpl in *; try solve[inv H0]; unfold_coerce;
-tc_assert_ext; auto;
-destruct (eval_expr e1 rho); destruct (eval_expr e2 rho); auto;
-simpl in *; destruct t; simpl in *; auto; unfold_coerce;
- tc_assert_ext; auto; repeat (try rewrite orb_if; rewrite andb_if);
-repeat (if_tac; auto). 
-Qed. 
-
-Lemma typecheck_xor_sound:
-forall (Delta : tycontext) (rho : environ) (e1 e2 : expr) (t : type),
-   denote_tc_assert (typecheck_expr Delta e2) rho ->
-   denote_tc_assert (isBinOpResultType Oxor e1 e2 t) rho ->
-   denote_tc_assert (typecheck_expr Delta e1) rho ->
-   typecheck_val (eval_expr e2 rho) (typeof e2) = true ->
-   typecheck_val (eval_expr e1 rho) (typeof e1) = true ->
-   typecheck_val
-     (eval_binop Oxor (typeof e1) (typeof e2) (eval_expr e1 rho)
-        (eval_expr e2 rho)) t = true.
-Proof. 
-intros. simpl in *; unfold eval_binop; unfold sem_binary_operation.
-unfold sem_xor in *. 
-destruct (typeof e1); destruct (typeof e2); simpl in *; auto;
-
-try destruct i; try destruct s; try destruct i0; try destruct s0; 
-simpl in *; try solve[inv H0]; unfold_coerce;
-tc_assert_ext; auto;
-destruct (eval_expr e1 rho); destruct (eval_expr e2 rho); auto;
-simpl in *; destruct t; simpl in *; auto; unfold_coerce;
- tc_assert_ext; auto; repeat (try rewrite orb_if; rewrite andb_if);
-repeat (if_tac; auto). 
-Qed. 
-
-Lemma typecheck_shl_sound:
-forall (Delta : tycontext) (rho : environ) (e1 e2 : expr) (t : type),
+Lemma typecheck_shift_sound:
+forall op (Delta : tycontext) (rho : environ) (e1 e2 : expr) (t : type)
+   (OPER: match op with Oshl | Oshr => True | _ => False end),
    denote_tc_assert (typecheck_expr Delta e2) rho ->
    denote_tc_assert (isBinOpResultType Oshl e1 e2 t) rho ->
    denote_tc_assert (typecheck_expr Delta e1) rho ->
    typecheck_val (eval_expr e2 rho) (typeof e2) = true ->
    typecheck_val (eval_expr e1 rho) (typeof e1) = true ->
    typecheck_val
-     (eval_binop Oshl (typeof e1) (typeof e2) (eval_expr e1 rho)
+     (eval_binop op (typeof e1) (typeof e2) (eval_expr e1 rho)
         (eval_expr e2 rho)) t = true.
 Proof. 
-intros. simpl in *; unfold eval_binop; unfold sem_binary_operation.
-unfold sem_shl in *. 
-destruct (typeof e1); destruct (typeof e2); simpl in *; auto;
+destruct op; try contradiction;
+abstract (
+intros; typecheck_sound_solver Delta rho e1 e2 t;
+unfold eval_binop; unfold sem_binary_operation, sem_shl, sem_shr; simpl;
+destruct (eval_expr e1 rho); inv H3;
+destruct (eval_expr e2 rho); inv H2;
+simpl; rewrite H0; reflexivity).
+Qed.
 
-try destruct i; try destruct s; try destruct i0; try destruct s0; 
-simpl in *; try solve[inv H0]; unfold_coerce;
- destruct t; simpl in *; auto; unfold_coerce;
-tc_assert_ext; auto;
-destruct (eval_expr e1 rho); destruct (eval_expr e2 rho); auto;
-simpl in *;
-unfold_coerce; tc_assert_ext; auto; repeat (try rewrite orb_if; rewrite andb_if);
-repeat (if_tac; auto). 
-Qed. 
+Lemma cmp_sound_aux:
+  forall b i s a , typecheck_val (force_val (Some (Val.of_bool b))) (Tint i s a) = true.
+Proof. destruct b; reflexivity. Qed.
 
-
-Lemma typecheck_shr_sound:
-forall (Delta : tycontext) (rho : environ) (e1 e2 : expr) (t : type),
+Lemma typecheck_cmp_sound:
+forall op (Delta : tycontext) (rho : environ) (e1 e2 : expr) (t : type)
+   (CMP:  match op with Oeq | One | Olt | Ogt | Ole | Oge => True | _ => False end),
    denote_tc_assert (typecheck_expr Delta e2) rho ->
-   denote_tc_assert (isBinOpResultType Oshr e1 e2 t) rho ->
+   denote_tc_assert (isBinOpResultType op e1 e2 t) rho ->
    denote_tc_assert (typecheck_expr Delta e1) rho ->
    typecheck_val (eval_expr e2 rho) (typeof e2) = true ->
    typecheck_val (eval_expr e1 rho) (typeof e1) = true ->
    typecheck_val
-     (eval_binop Oshr (typeof e1) (typeof e2) (eval_expr e1 rho)
+     (eval_binop op (typeof e1) (typeof e2) (eval_expr e1 rho)
         (eval_expr e2 rho)) t = true.
-Proof. 
-intros. simpl in *; unfold eval_binop; unfold sem_binary_operation.
-unfold sem_shr in *. 
-destruct (typeof e1); destruct (typeof e2); simpl in *; auto;
-
-try destruct i; try destruct s; try destruct i0; try destruct s0; 
-simpl in *; try solve[inv H0]; unfold_coerce;
- destruct t; simpl in *; auto; unfold_coerce;
-tc_assert_ext; auto;
-destruct (eval_expr e1 rho); destruct (eval_expr e2 rho); auto;
-simpl in *;
-unfold_coerce; tc_assert_ext; auto; repeat (try rewrite orb_if; rewrite andb_if);
-repeat (if_tac; auto). 
-Qed. 
-
-
-Lemma typecheck_eq_sound:
-forall (Delta : tycontext) (rho : environ) (e1 e2 : expr) (t : type),
-   denote_tc_assert (typecheck_expr Delta e2) rho ->
-   denote_tc_assert (isBinOpResultType Oeq e1 e2 t) rho ->
-   denote_tc_assert (typecheck_expr Delta e1) rho ->
-   typecheck_val (eval_expr e2 rho) (typeof e2) = true ->
-   typecheck_val (eval_expr e1 rho) (typeof e1) = true ->
-   typecheck_val
-     (eval_binop Oeq (typeof e1) (typeof e2) (eval_expr e1 rho)
-        (eval_expr e2 rho)) t = true.
-Proof. 
-intros. simpl in *; unfold eval_binop; unfold sem_binary_operation.
-unfold sem_cmp in *. 
-destruct (typeof e1); destruct (typeof e2); simpl in *; auto;
-
-try destruct i; try destruct s; try destruct i0; try destruct s0; 
-simpl in *; try solve[inv H0]; unfold_coerce;
-tc_assert_ext; auto;
-destruct (eval_expr e1 rho); destruct (eval_expr e2 rho); auto;
-simpl in *; destruct t; simpl in *; auto; unfold_coerce;
-unfold_coerce; tc_assert_ext; auto; repeat (try rewrite orb_if; rewrite andb_if);
-repeat (if_tac; auto); of_bool_destruct; auto. 
-Qed. 
-
-Lemma typecheck_ne_sound:
-forall (Delta : tycontext) (rho : environ) (e1 e2 : expr) (t : type),
-   denote_tc_assert (typecheck_expr Delta e2) rho ->
-   denote_tc_assert (isBinOpResultType One e1 e2 t) rho ->
-   denote_tc_assert (typecheck_expr Delta e1) rho ->
-   typecheck_val (eval_expr e2 rho) (typeof e2) = true ->
-   typecheck_val (eval_expr e1 rho) (typeof e1) = true ->
-   typecheck_val
-     (eval_binop One (typeof e1) (typeof e2) (eval_expr e1 rho)
-        (eval_expr e2 rho)) t = true.
-Proof. 
-intros. simpl in *; unfold eval_binop; unfold sem_binary_operation.
-unfold sem_cmp in *. 
-destruct (typeof e1); destruct (typeof e2); simpl in *; auto;
-
-try destruct i; try destruct s; try destruct i0; try destruct s0; 
-simpl in *; try solve[inv H0]; unfold_coerce;
-tc_assert_ext; auto;
-destruct (eval_expr e1 rho); destruct (eval_expr e2 rho); auto;
-simpl in *; destruct t; simpl in *; auto; unfold_coerce;
- tc_assert_ext; auto; repeat (try rewrite orb_if; rewrite andb_if);
-repeat (if_tac; auto); of_bool_destruct; auto. 
-Qed. 
-
-Lemma typecheck_lt_sound:
-forall (Delta : tycontext) (rho : environ) (e1 e2 : expr) (t : type),
-   denote_tc_assert (typecheck_expr Delta e2) rho ->
-   denote_tc_assert (isBinOpResultType Olt e1 e2 t) rho ->
-   denote_tc_assert (typecheck_expr Delta e1) rho ->
-   typecheck_val (eval_expr e2 rho) (typeof e2) = true ->
-   typecheck_val (eval_expr e1 rho) (typeof e1) = true ->
-   typecheck_val
-     (eval_binop Olt (typeof e1) (typeof e2) (eval_expr e1 rho)
-        (eval_expr e2 rho)) t = true.
-Proof. 
-intros. simpl in *; unfold eval_binop; unfold sem_binary_operation.
-unfold sem_cmp in *. 
-destruct (typeof e1); destruct (typeof e2); simpl in *; auto;
-
-try destruct i; try destruct s; try destruct i0; try destruct s0; 
-simpl in *; try solve[inv H0]; unfold_coerce;
-tc_assert_ext; auto;
-destruct (eval_expr e1 rho); destruct (eval_expr e2 rho); auto;
-simpl in *; destruct t; simpl in *; auto; unfold_coerce;
- tc_assert_ext; auto; repeat (try rewrite orb_if; rewrite andb_if);
-repeat (if_tac; auto); of_bool_destruct; auto. 
-Qed. 
-
-Lemma typecheck_le_sound:
-forall (Delta : tycontext) (rho : environ) (e1 e2 : expr) (t : type),
-   denote_tc_assert (typecheck_expr Delta e2) rho ->
-   denote_tc_assert (isBinOpResultType Ole e1 e2 t) rho ->
-   denote_tc_assert (typecheck_expr Delta e1) rho ->
-   typecheck_val (eval_expr e2 rho) (typeof e2) = true ->
-   typecheck_val (eval_expr e1 rho) (typeof e1) = true ->
-   typecheck_val
-     (eval_binop Ole (typeof e1) (typeof e2) (eval_expr e1 rho)
-        (eval_expr e2 rho)) t = true.
-Proof. 
-intros. simpl in *; unfold eval_binop; unfold sem_binary_operation.
-unfold sem_cmp in *. 
-destruct (typeof e1); destruct (typeof e2); simpl in *; auto;
-
-try destruct i; try destruct s; try destruct i0; try destruct s0; 
-simpl in *; try solve[inv H0]; unfold_coerce;
-tc_assert_ext; auto;
-destruct (eval_expr e1 rho); destruct (eval_expr e2 rho); auto;
-simpl in *; destruct t; simpl in *; auto; unfold_coerce;
- tc_assert_ext; auto; repeat (try rewrite orb_if; rewrite andb_if);
-repeat (if_tac; auto); of_bool_destruct; auto. 
-Qed. 
-
-Lemma typecheck_gt_sound:
-forall (Delta : tycontext) (rho : environ) (e1 e2 : expr) (t : type),
-   denote_tc_assert (typecheck_expr Delta e2) rho ->
-   denote_tc_assert (isBinOpResultType Ogt e1 e2 t) rho ->
-   denote_tc_assert (typecheck_expr Delta e1) rho ->
-   typecheck_val (eval_expr e2 rho) (typeof e2) = true ->
-   typecheck_val (eval_expr e1 rho) (typeof e1) = true ->
-   typecheck_val
-     (eval_binop Ogt (typeof e1) (typeof e2) (eval_expr e1 rho)
-        (eval_expr e2 rho)) t = true.
-Proof. 
-intros. simpl in *; unfold eval_binop; unfold sem_binary_operation.
-unfold sem_cmp in *. 
-destruct (typeof e1); destruct (typeof e2); simpl in *; auto;
-
-try destruct i; try destruct s; try destruct i0; try destruct s0; 
-simpl in *; try solve[inv H0]; unfold_coerce;
-tc_assert_ext; auto;
-destruct (eval_expr e1 rho); destruct (eval_expr e2 rho); auto;
-simpl in *; destruct t; simpl in *; auto; unfold_coerce;
- tc_assert_ext; auto; repeat (try rewrite orb_if; rewrite andb_if);
-repeat (if_tac; auto); of_bool_destruct; auto. 
-Qed. 
-
-Lemma typecheck_ge_sound:
-forall (Delta : tycontext) (rho : environ) (e1 e2 : expr) (t : type),
-   denote_tc_assert (typecheck_expr Delta e2) rho ->
-   denote_tc_assert (isBinOpResultType Oge e1 e2 t) rho ->
-   denote_tc_assert (typecheck_expr Delta e1) rho ->
-   typecheck_val (eval_expr e2 rho) (typeof e2) = true ->
-   typecheck_val (eval_expr e1 rho) (typeof e1) = true ->
-   typecheck_val
-     (eval_binop Oge (typeof e1) (typeof e2) (eval_expr e1 rho)
-        (eval_expr e2 rho)) t = true.
-Proof. 
-intros. simpl in *; unfold eval_binop; unfold sem_binary_operation.
-unfold sem_cmp in *. 
-destruct (typeof e1); destruct (typeof e2); simpl in *; auto;
-
-try destruct i; try destruct s; try destruct i0; try destruct s0; 
-simpl in *; try solve[inv H0]; unfold_coerce;
-tc_assert_ext; auto;
-destruct (eval_expr e1 rho); destruct (eval_expr e2 rho); auto;
-simpl in *; destruct t; simpl in *; auto; unfold_coerce;
- tc_assert_ext; auto; repeat (try rewrite orb_if; rewrite andb_if);
-repeat (if_tac; auto); of_bool_destruct; auto. 
-Qed. 
-
+Proof.
+intros.
+destruct op; try (contradiction CMP);
+abstract (intros; typecheck_sound_solver Delta rho e1 e2 t;
+unfold eval_binop; unfold sem_binary_operation, sem_cmp; simpl;
+destruct (eval_expr e1 rho); inv H3;
+destruct (eval_expr e2 rho); inv H2;
+apply cmp_sound_aux).
+Qed.
 
 Lemma typecheck_binop_sound:
 forall (Delta : tycontext) (rho : environ) (b : binary_operation)
@@ -408,25 +151,14 @@ typecheck_val (eval_expr (Ebinop b e1 e2 t) rho) (typeof (Ebinop b e1 e2 t)) =
 true.
 Proof. 
 intros. simpl in *.  rewrite tc_andp_sound in H. 
-simpl in *. unfold_coerce; rewrite tc_andp_sound in H. 
-simpl in *. unfold_coerce; intuition.  
-destruct b. 
-eapply typecheck_add_sound; eauto.  
-eapply typecheck_sub_sound; eauto.
-eapply typecheck_mul_sound; eauto.
-eapply typecheck_div_sound; eauto.
-eapply typecheck_mod_sound; eauto.
-eapply typecheck_and_sound; eauto.
-eapply typecheck_or_sound; eauto.
-eapply typecheck_xor_sound; eauto.
-eapply typecheck_shl_sound; eauto.
-eapply typecheck_shr_sound; eauto.
-eapply typecheck_eq_sound; eauto.
-eapply typecheck_ne_sound; eauto.
-eapply typecheck_lt_sound; eauto.
-eapply typecheck_gt_sound; eauto.
-eapply typecheck_le_sound; eauto. 
-eapply typecheck_ge_sound; eauto. 
+simpl in *. super_unfold_lift; rewrite tc_andp_sound in H. 
+simpl in *. super_unfold_lift; intuition.  
+destruct b;
+try (eapply typecheck_sub_sound; eauto);
+try solve [eapply typecheck_divmod_sound; simpl; eauto];
+try solve [eapply typecheck_shift_sound; simpl; eauto];
+try solve [eapply typecheck_cmp_sound; simpl; eauto];
+try solve [abstract (typecheck_sound_solver Delta rho e1 e2 t)].
 Qed.
 
 
