veric/lift.v
@@ -1,0 +1,140 @@
+(* Lifted functions.
+   By Jesper Bengtson, revised by Andrew W. Appel.
+*)
+
+Structure Lift := mkLift {
+         lift_S: Type;
+         lift_T: Type; 
+         lift_prod : Type;
+         lift_last: Type;
+         lifted:> Type;
+         lift_curry: lift_T -> lift_prod -> lift_last;
+         lift_uncurry_open: ((lift_S -> lift_prod) -> (lift_S -> lift_last)) -> lifted
+}.
+          
+Definition Tend (S: Type) (A: Type) := 
+    mkLift S A unit A 
+          (S -> A)
+          (fun f _ => f)
+          (fun f => f (fun _: S => tt)).
+
+Canonical Structure Tarrow (A: Type) (H: Lift) := 
+    mkLift (lift_S H)
+      (A -> lift_T H) 
+      (prod A (lift_prod H))
+      (lift_last H)
+      ((lift_S H -> A) -> lifted H)
+      (fun f x => match x with (x1,x2) => lift_curry H (f x1) x2 end)
+      (fun f x => lift_uncurry_open H (fun y: lift_S H -> lift_prod H => f (fun z => (x z, y z)))).
+
+Set Implicit Arguments.
+Unset Strict Implicit.
+Set Maximal Implicit Insertion.
+
+Definition lift S {A B} (f : A -> B) (a : S -> A) (x: S) : B := f (a x).
+
+Definition liftx' {H: Lift} (f: lift_T H) : lifted H :=
+  lift_uncurry_open H (lift (lift_curry H f)).
+
+Definition liftx {H: Lift} (f: lift_T H) : lifted H :=   @liftx' H f.
+Opaque liftx.
+
+(* NOTE: We want unfold_lift to unfold EVERYTHING related to lifting, but NOTHING else.
+  Thus we have avoided using any library functions to implement lifting, so that
+  we can unfold all of it without interfering with other things the user might be doing. *)
+
+Definition id_for_lift {A} (x: A) := x. (* Obsolete? way of getting
+          `(fun x: A => ...x...) to work. Not in active use right now. *)
+
+Tactic Notation "unfold_lift" := 
+  change @liftx with @liftx'; unfold liftx' (*, id_for_lift*);
+  repeat match goal with(* This unfolds instances of Tend *)
+  | |- context [lift_uncurry_open (?F _)] => unfold F 
+  | |- context [Tarrow _ (?F _)] => unfold F 
+  end;
+  unfold Tarrow, Tend, lift_S, lift_T, lift_prod, lift_last, lifted, lift_uncurry_open, lift_curry, lift.
+
+Tactic Notation "unfold_lift" "in" hyp(H) := (* move this to veric/lift.v *)
+  change @liftx with @liftx' in H;  unfold liftx' (*, id_for_lift*) in H;
+  repeat match type of H with(* This unfolds instances of Tend *)
+  | context [lift_uncurry_open (?F _)] => unfold F in H
+  | context [Tarrow _ (?F _)] => unfold F in H
+  end;
+  unfold liftx', Tarrow, Tend, lift_S, lift_T, lift_prod, lift_last, lifted, lift_uncurry_open, lift_curry, lift in H.
+
+Tactic Notation "unfold_lift" "in" "*" :=
+  change @liftx with @liftx' in *;  unfold liftx' (*, id_for_lift *) in *;
+  repeat match goal with (* This unfolds instances of Tend *)
+             | H: context [lift_uncurry_open (?F _)] |- _ => unfold F in H
+             | |- context [Tarrow _ (?F _)] => unfold F 
+             end; 
+  unfold liftx', Tarrow, Tend, lift_S, lift_T, lift_prod, lift_last, lifted, lift_uncurry_open, lift_curry, lift in *.
+
+
+(* The reaspon for writing   liftx(x : _) instead 
+  of just (liftx x)  is to get the case  `(fun v => ..v...) to work *)
+Notation "'`' x" := (liftx x) (at level 9).
+Notation "'`(' x ')'" := (liftx (x : _)).
+
+(*  EXAMPLES OF USE
+
+Parameter environ : Type.
+
+Canonical Structure LiftEnviron := Tend environ.
+
+Definition foo (v : nat) := (v=O).
+Check (`foo).
+Check (`(fun v => v=O)).
+
+(* Infix "-.>" := Tarrow (at level 80, right associativity).  (* The
+      only purpose of this Infix is to make the error message slightly prettier,
+      but they're not bad even without it. *) *)
+(* Notation  "x '-.>[' y ] " := (Tarrow x (LiftEnviron y)) (at level 80, right associativity).  *)
+
+
+Check `plus.
+Check (`(plus 4)).
+
+(* Goal (lifted (nat -.> (nat -.> LiftEnviron nat)) = ((environ -> nat) -> (environ -> nat) -> (environ -> nat))).
+reflexivity.
+Qed.
+*)
+
+Parameter f: environ -> nat.
+Check (`plus f).
+Check (`plus f f).
+Check (`(@cons nat)).
+Check (`(@cons nat) (`plus f f) `nil).
+Check (`(@cons _) (`plus f f) `nil).     (* HA!  This line would not have worked using typeclasses for Lift; 
+            it does work using canonical structures *)
+(* Check (`cons (`plus f f) `nil).     (* this line fails, which is OK; however, using the old 'coerce' appoach,
+                                                           this would have worked.  *) *)
+
+
+Example test_plus (s : environ) : (`plus `(4) `3) s = (`(7)) s.
+  simpl.  (* doesn't unfold the backtick; this is a good thing, I think. *)
+ unfold_lift. (* optional -- proof works with or without it *)  
+  reflexivity.
+Qed.
+
+Example test_plus' (s : environ) : (`plus `(4) `3) s = (`(7)) s.
+  simpl.  (* doesn't unfold the backtick; this is a good thing, I think. *)
+  reflexivity.
+Qed.
+
+Definition natfun := nat -> nat.
+Opaque natfun.
+
+Definition add : nat -> natfun := plus.
+
+Goal forall rho, `add `(3) rho = (fun y => plus 3 y).
+ intro rho.
+ simpl.  (* doesn't unfold the backtick; this is a good thing, I think. *)
+ unfold_lift. (* optional -- see what happens! *)
+ reflexivity.
+Qed.
+
+(* Goal `add `3 = `plus `3.   (* This fails.  Indeed, it should fail.  
+       But the error message is reasonably informative! *)  *)
+
+END EXAMPLES OF USE *)
