veric/semax_call.v
@@ -414,7 +414,7 @@ destruct H0 as [v [loc [[? ?] ?]]].
  destruct H1 as [? ?].
 exists v; exists loc; split; auto.
 split; auto.
-destruct fs.
+destruct fs as [f A a a0].
 simpl in H4|-*.
 pose proof (necR_resource_at (core w) (core w') loc
          (PURE (FUN f) (SomeP (A :: boolT :: environ :: nil) (packPQ a a0))) CORE).
@@ -523,7 +523,7 @@ destruct fsig. unfold fn_funsig in *. inversion H3; clear H3; subst l t. simpl i
  revert vl H H0; induction bl; destruct vl; intros; inv H0; simpl.
  constructor.
  destruct p. simpl in *; subst.
- repeat (rewrite tc_andp_sound in *; simpl in *; unfold_coerce).
+ repeat (rewrite tc_andp_sound in *; simpl in *; super_unfold_lift).
  destruct H as [[? ?] ?].
  pose proof (typecheck_expr_sound _ _ _ H1 H).
  specialize (IHbl _ H2 H4).
@@ -695,7 +695,7 @@ induction (fn_params f); intros.  inv H. simpl in *.
 destruct a. simpl in *. remember (split l). destruct p. 
 simpl in *. destruct H. clear IHl. destruct bl. inv H.  inv Heqp. inv TC2.   
 inv H. inv Heqp. simpl in *. 
- repeat (rewrite tc_andp_sound in *; simpl in *; unfold_coerce).
+ repeat (rewrite tc_andp_sound in *; simpl in *; super_unfold_lift).
 destruct TC2 as [[? ?] ?].
 rewrite (pass_params_ni _ _ id _ _ H21) by (inv H17; contradict H4; apply in_app; auto).
 rewrite PTree.gss.
@@ -712,8 +712,8 @@ auto. auto. inv Heqp.
 destruct bl.  inv TC2. 
 inv H17.
 simpl in *.  
- repeat (rewrite tc_andp_sound in *; simpl in *; unfold_coerce).
-unfold_coerce. destruct TC2 as [[? ?] ? ].
+ repeat (rewrite tc_andp_sound in *; simpl in *; super_unfold_lift).
+super_unfold_lift. destruct TC2 as [[? ?] ? ].
 assert (i <> id). intuition. subst. apply H2. apply in_or_app. left.
 apply in_map with (f := fst) in H. apply H.
 
@@ -1591,7 +1591,7 @@ econstructor; try eassumption; simpl.
 exists (eval_expr e (construct_rho (filter_genv psi) ve te)).
 assert (TCe: denote_tc_assert (typecheck_expr Delta e)  (construct_rho (filter_genv psi) ve te)).
 simpl in *. 
- repeat (rewrite tc_andp_sound in *; simpl in *; unfold_coerce).
+ repeat (rewrite tc_andp_sound in *; simpl in *; super_unfold_lift).
 destruct TC; auto.
 split.
 apply eval_expr_relate with (Delta := Delta); auto.
@@ -1600,13 +1600,13 @@ destruct H3.
 simpl in H6; rewrite (call_cont_current_function H7) in H6.
 destruct H6 as [_ ?].
 rewrite H6.
-unfold eval_cast. unfold_coerce.
+unfold eval_cast. super_unfold_lift.
 apply cast_exists with Delta; auto.
 
 auto.
 rewrite <- H6.
 simpl in TC. 
- repeat (rewrite tc_andp_sound in *; simpl in *; unfold_coerce).
+ repeat (rewrite tc_andp_sound in *; simpl in *; super_unfold_lift).
 destruct TC; auto.
 
 inv H9.
@@ -1621,7 +1621,7 @@ destruct H10 as [_ H10]. rewrite H6 in H10.
 rewrite H10 in TC.
 clear - TC.
 simpl in TC.
- repeat (rewrite tc_andp_sound in *; simpl in *; unfold_coerce).
+ repeat (rewrite tc_andp_sound in *; simpl in *; super_unfold_lift).
 destruct TC as [_ ?].
 apply H. 
 simpl.
